Further cleanup for the AV instantiation of the abstract transition system

src/theory/tools/wp/bin_hoare_logic_test_AVScript.sml
@@ -4,221 +4,54 @@ open bir_programTheory;
 open bir_auxiliaryTheory;
 open bin_hoare_logicTheory;
 open bir_program_multistep_propsTheory;
+open bir_program_terminationTheory;
 open bir_program_blocksTheory;
+
+open bin_hoare_logic_testTheory;
 
 open bir_auxiliaryLib;
 
 open HolBACoreSimps;
-
+open bin_hoare_logicSimps;
+(* TODO: Have this depend on bin_hoare_logic_testScript.sml? *)
 val _ = new_theory "bin_hoare_logic_test_AV";
 
+(******************************************************************)
+(*                         DEFINITIONS                            *)
+(******************************************************************)
+
+(* TODO: Try bir_exec_to_addr_label - but this could cause more
+ * problems *)
+(* TODO: For now, this is the same as in
+ * bin_hoare_logic_testScript.sml *)
 (*
-(* Executing till a certain set of labels is useful as well. Since we might loop
-   outside this set of labels, infinite runs are possible. *)
-val bir_exec_to_labels_n_def = Define `
-  bir_exec_to_labels_n ls p state n =
-  bir_exec_steps_GEN (F, \pc. (pc.bpc_index = 0) /\ (pc.bpc_label IN ls)) p state (SOME n)`
-
-val bir_exec_to_labels_def = Define `
-  bir_exec_to_labels ls p state = bir_exec_to_labels_n ls p state 1`
-*)
-
-(*
-Datatype `bin_model_t =
-  <|(* A function to obtain a state option from a state via
-     * execution (transition) *)
-    trs : 'a -> 'a option;
-    (* A function to determine whether a transition between two
-     * states is OK, through using a set of labels for which
-     * execution must halt if reached, meaning they cannot be
-     * touched in any intermediate step *)
-    weak : 'a -> ('b -> bool) -> 'a -> bool;
-    (* A function to obtain the program counter from a state *)
-    pc : 'a -> 'b
-   |>`;
-
-*)
-
-(*
-val weak_model_def = Define `
-  weak_model m =
-    !ms ls ms'.
-      (m.weak ms ls ms') =
-        ?n.
-          ((n > 0) /\
-           (FUNPOW_OPT m.trs n ms = SOME ms') /\
-           ((m.pc ms') IN ls)
-          ) /\
-          !n'.
-            (((n' < n) /\ (n' > 0)) ==>
-            ?ms''.
-              (FUNPOW_OPT m.trs n' ms = SOME ms'') /\
-              (~((m.pc ms'') IN ls))
-            )`;
-*)
-
-(* TODO: bir_exec_block_n should probably return a BER_Ended or a
- * BER_Looping... *)
-(* Try bir_exec_to_addr_label - but could cause more problems *)
-(*
-val bir_trs_def = Define `
-  bir_trs prog ms =
-  SOME (
-    SND (
-      SND (
-        SND (bir_exec_block_n prog ms 1)
-      )
-    )
-  )`;
-*)
-val bir_trs_def = Define `
-  bir_trs (prog:'a bir_program_t) ms =
+val bir_trs_av_def = Define `
+  bir_trs_av (prog:'a bir_program_t) st =
   let
-    (_, _, _, st) = bir_exec_block_n prog ms 1
+    (_, _, _, st') = bir_exec_block_n prog st 1
   in
-   if st.bst_status = BST_Running
-   then SOME st
+   if ~(bir_state_is_terminated st')
+   then SOME st'
    else NONE
 `;
-
-(* TODO: Move elsewhere... *)
-val bir_get_current_statement_EMPTY =
-  store_thm("bir_get_current_statement_EMPTY",
-  ``!pc.
-      bir_get_current_statement (BirProgram []) pc = NONE``,
-
-FULL_SIMP_TAC (std_ss++holBACore_ss)
-              [bir_get_current_statement_def,
-               bir_get_program_block_info_by_label_def,
-               listTheory.INDEX_FIND_def]
-);
-
-val bir_exec_block_n_EXISTS = store_thm("bir_exec_block_n_EXISTS",
-  ``!prog ms.
-      ?a b c d.
-        bir_exec_block_n prog ms 1 = (a, b, c, d)``,
-
-REPEAT STRIP_TAC >>
-Cases_on `bir_state_is_terminated ms` >- (
-  FULL_SIMP_TAC std_ss [bir_exec_block_n_REWR_TERMINATED]
-) >>
-FULL_SIMP_TAC std_ss [bir_exec_block_n_TO_steps_GEN,
-                      bir_exec_steps_GEN_1_EQ_Ended] >>
-cheat
-(* Proof sketch from here:
-   Either the PC of state ms points to a block in prog, or it does
-   not. If it does not, we are OK, since any execution will result
-   in Failed, terminating and yielding an Ended result.
-
-   If the PC of state ms points to some block in prog, then do
-   induction the list of basic statements: For the empty list, the
-   PC must point to the ending statement. Consider the cases: if the
-   ending statement is Halt, we are OK. If the ending statement is
-   a CJmp whose condition fails to evaluate, we are OK. If the
-   ending statement jumps outside the program, we are OK, since
-   this will cause JumpOutside, which is a terminating state. In
-   the case of jumps inside the program, there exist two
-   possibilities: either jumps to other blocks (OK) or jumps to the
-   same block, which will not give a Looping result, but will make
-   pc_cond trigger.
-
-   For every basic statement in a non-empty list, we will either
-   terminate (by violating Assertions or Assumptions), in which case
-   we are OK, or we will proceed to executing the next basic
-   statement, or the ending statement (in which case the proof is
-   same as above).
-
 *)
-(* OLD:
-Cases_on `prog` >>
-Cases_on `l` >- (
-  (* Case: Empty program *)
-  (* TODO: Lemma about empty program? *)
-  FULL_SIMP_TAC std_ss [bir_exec_infinite_steps_fun_def] >>
-  EXISTS_TAC ``1:num`` >>
-  EXISTS_TAC ``0:num`` >>
-  FULL_SIMP_TAC std_ss [arithmeticTheory.FUNPOW_1,
-                        bir_exec_step_state_def,
-                        bir_exec_step_def,
-                        arithmeticTheory.FUNPOW] >>
-  CONJ_TAC >- (
-    FULL_SIMP_TAC (std_ss++holBACore_ss)
-                  [bir_state_COUNT_PC_def,
-                   bir_get_current_statement_EMPTY,
-                   bir_state_set_failed_def],
-  ) >>
-  CONJ_TAC >- (
-    FULL_SIMP_TAC (std_ss++holBACore_ss)
-                  [bir_get_current_statement_EMPTY,
-                   bir_state_set_failed_def]
-  ) >>
-  CONJ_TAC >- (
-    REPEAT STRIP_TAC >>
-    (* TODO: Lemma stating that n < 1 ==> n = 0 ??? *)
-    Cases_on `n` >| [
-      FULL_SIMP_TAC (std_ss++holBACore_ss)
-		    [arithmeticTheory.FUNPOW],
 
-      FULL_SIMP_TAC arith_ss []
-    ]
-  ) >>
-  FULL_SIMP_TAC arith_ss []
-) >>
-  (* Case: Program nonempty. *)
-  FULL_SIMP_TAC std_ss [bir_exec_infinite_steps_fun_def] >>
-  Cases_on `h` >>
-  Cases_on `l` >| [
-    (* Case: Statement list empty *)
-    EXISTS_TAC ``1:num`` >> (* First witness is 1 in both cases *)
-    FULL_SIMP_TAC std_ss [arithmeticTheory.FUNPOW_1,
-                          bir_exec_step_state_def,
-                          bir_exec_step_def] >>
-    Cases_on `bir_get_current_statement (BirProgram (bir_block_t b [] b0::t)) ms.bst_pc` >| [
-      FULL_SIMP_TAC (std_ss++holBACore_ss)
-                    [bir_state_set_failed_def,
-                     bir_state_COUNT_PC_def] >>
-      FULL_SIMP_TAC arith_ss [] >>
-      REPEAT STRIP_TAC >>
-      Cases_on `n` >| [
-	FULL_SIMP_TAC (std_ss++holBACore_ss)
-		      [arithmeticTheory.FUNPOW],
-
-	FULL_SIMP_TAC arith_ss []
-      ],
-
-      (* Case: Current statement is something *)
-      FULL_SIMP_TAC (std_ss++holBACore_ss) [bir_exec_stmt_def]
-      Induct_on `x`
-    ]
-
-    (* Case: Statement list non-empty. Needed to show that it is
-     * OK with termination on every statement, but quantifiers must
-     * be instantiated with this in mind... *)
-
-      (* Case of non-termination would also require a case split on
-       * the ending statement causing termination? *)
-  ]
-  (* Should be length of block h... *)
-  EXISTS_TAC ``((LENGTH (l:'a bir_stmt_basic_t list)) + 1):num`` >> 
-  EXISTS_TAC ``1:num`` >>
-  cheat
-*)
-);
-
-val _ = Datatype `bir_weak_state =
+val _ = Datatype `bir_weak_state_t =
     BWS_Regular bir_label_t
   | BWS_Top
   | BWS_Bottom
 `;
 
+
 val bir_get_weak_state_def = Define `
-  bir_get_weak_state bir_state =
-    if bir_state.bst_status = BST_Running
-    then BWS_Regular (bir_state.bst_pc.bpc_label)
-    else if bir_state.bst_status = BST_AssumptionViolated
+  bir_get_weak_state st =
+    if ~(bir_state_is_terminated st)
+    then BWS_Regular (st.bst_pc.bpc_label)
+    else if st.bst_status = BST_AssumptionViolated
     then BWS_Top
     else BWS_Bottom
 `;
+
 
 val bir_get_label_from_weak_state_def = Define `
   bir_get_label_from_weak_state ws =
@@ -235,223 +68,269 @@ val bir_get_label_set_from_weak_state_set_no_top_def = Define `
     )
 `;
 
-val bir_weak_trs_def = Define `
-  bir_weak_trs wss prog ms =
+
+val bir_weak_trs_av_def = Define `
+  bir_weak_trs_av wss prog st =
     let 
       ls = bir_get_label_set_from_weak_state_set_no_top wss
     in
-    case (bir_exec_to_labels ls prog ms) of
-      BER_Ended _ _ _ bir_state =>
-        if ((bir_get_weak_state bir_state) IN wss)
-        then SOME bir_state
+    case (bir_exec_to_labels ls prog st) of
+      BER_Ended _ _ _ st' =>
+        if ((bir_get_weak_state st') IN wss)
+        then SOME st'
         else NONE
     | BER_Looping _ => NONE
 `;
 
-(* 1. Instantiate a new weak model *)
-val bir_etl_wm_def =
-  Define `bir_etl_wm (prog :'a bir_program_t) = <|
+
+(* The BIR WM which is later proven to obey the property
+ * "weak_model". *)
+val bir_etl_wm_av_def =
+  Define `bir_etl_wm_av (prog :'a bir_program_t) = <|
     trs  := bir_trs prog;
-    weak := (\ms wss ms'.
-	       (bir_weak_trs wss prog ms = SOME ms')
+    weak := (\st wss st'.
+	       (bir_weak_trs_av wss prog st = SOME st')
 	    );
-    pc   := (\ms. bir_get_weak_state ms)
+    pc   := (\st. bir_get_weak_state st)
   |>`;
 
-val wm_type = mk_thy_type {Tyop="bin_model_t",
-                           Thy="bin_hoare_logic",
-                           Args=[``:bir_state_t``,
-                                 ``:bir_label_t``]
+
+(******************************************************************)
+(*                            LEMMATA                             *)
+(******************************************************************)
+
+local
+
+val ws_type = mk_thy_type {Tyop="bir_weak_state_t",
+                           Thy="bin_hoare_logic_test_AV",
+                           Args=[]
                           };
 
-val bir_wm_SS = rewrites (flatten (map type_rws [wm_type]));
+val bir_ws_SS = rewrites (flatten (map type_rws [ws_type]));
 
-(* TODO: Move elsewhere... *)
-val bir_get_current_statement_NONE_stmt =
-  store_thm("bir_get_current_statement_NONE_stmt",
-  ``!prog pc.
-      (bir_get_current_statement prog pc = NONE) ==>
-      (bir_get_current_block prog pc = NONE)
-    ``,
+in
 
-FULL_SIMP_TAC (std_ss++holBACore_ss)
-              [bir_get_current_block_def,
-               bir_get_current_statement_def] >>
+val bir_ls_filter_keeps_regular =
+  store_thm("bir_ls_filter_keeps_regular",
+  ``!st ls.
+    st.bst_pc.bpc_label NOTIN
+      bir_get_label_set_from_weak_state_set_no_top ls <=>
+    BWS_Regular st.bst_pc.bpc_label NOTIN ls``,
+
 REPEAT STRIP_TAC >>
-Cases_on `bir_get_program_block_info_by_label
-            prog pc.bpc_label` >> (
-  FULL_SIMP_TAC (std_ss++holBACore_ss) []
-) >>
-Cases_on `x` >>
-Cases_on `0 = LENGTH r.bb_statements` >>
-Cases_on `0 < LENGTH r.bb_statements` >> (
-FULL_SIMP_TAC arith_ss []
-)
+EQ_TAC >| [
+  REPEAT STRIP_TAC >>
+  FULL_SIMP_TAC std_ss
+    [bir_get_label_set_from_weak_state_set_no_top_def,
+     pred_setTheory.IMAGE_IN, pred_setTheory.IMAGE_DEF] >>
+  REV_FULL_SIMP_TAC (std_ss++pred_setLib.PRED_SET_ss) [] >>
+  QSPECL_X_ASSUM ``!x. _`` [`SOME st.bst_pc.bpc_label`] >>
+  FULL_SIMP_TAC std_ss [] >>
+  QSPECL_X_ASSUM ``!x'. _`` [`BWS_Regular st.bst_pc.bpc_label`] >>
+  FULL_SIMP_TAC (std_ss++bir_ws_SS)
+    [bir_get_label_from_weak_state_def],
+
+  REPEAT STRIP_TAC >>
+  FULL_SIMP_TAC std_ss
+    [bir_get_label_set_from_weak_state_set_no_top_def,
+     pred_setTheory.IMAGE_IN, pred_setTheory.IMAGE_DEF] >>
+  REV_FULL_SIMP_TAC (std_ss++pred_setLib.PRED_SET_ss) [] >>
+  FULL_SIMP_TAC (std_ss++bir_ws_SS)
+    [bir_get_label_from_weak_state_def] >>
+  Cases_on `x'` >>
+  FULL_SIMP_TAC (std_ss++bir_ws_SS) []
+]
 );
 
+end
+
+(******************************************************************)
+(*                         MAIN PROOF                             *)
+(******************************************************************)
+
 (* 2. Prove that weak_model bir_etl_wm *)
-val bir_model_is_weak = store_thm("bir_model_is_weak",
+val bir_model_av_is_weak = store_thm("bir_model_av_is_weak",
   ``!(prog: 'a bir_program_t).
-      weak_model (bir_etl_wm prog)``,
+      weak_model (bir_etl_wm_av prog)``,
 
 REPEAT STRIP_TAC >>
 FULL_SIMP_TAC (std_ss++bir_wm_SS)
-              [weak_model_def, bir_etl_wm_def] >>
-FULL_SIMP_TAC std_ss [bir_weak_trs_def, LET_DEF] >>
+              [weak_model_def, bir_etl_wm_av_def] >>
+FULL_SIMP_TAC std_ss [bir_weak_trs_av_def, bir_get_weak_state_def,
+                      LET_DEF] >>
 REPEAT STRIP_TAC >>
 CASE_TAC >| [
   (* Case 1: Result of bir_exec_to_labels is Ended *)
-  CASE_TAC >| [
-    (* Case 1A: Weak state counterpart of b is in ls *)
-    FULL_SIMP_TAC std_ss [bir_exec_to_labels_def] >>
-    IMP_RES_TAC bir_exec_to_labels_n_TO_bir_exec_block_n >>
-    EQ_TAC >| [
-      (* Part one: Assuming b = ms', show bir_trs plays nice *)
-      REPEAT DISCH_TAC >>
-      (* subsume b... *)
-      Q.PAT_X_ASSUM `b = ms'`
-                    (fn thm => FULL_SIMP_TAC std_ss [thm]) >>
-      FULL_SIMP_TAC std_ss [bir_exec_to_labels_n_def,
-                            bir_exec_steps_GEN_SOME_EQ_Ended] >>
-      EXISTS_TAC ``m:num`` >>
-      (* TODO: Make lemma... *)
-      subgoal `!prog ms m l n c_l' ms'.
-        (bir_exec_block_n prog ms m = (l,n,c_l',ms')) ==>
-        ?m'.
-        (FUNPOW_OPT (bir_trs prog) m' ms = SOME ms')` >- (
-        cheat
-      ) >>
-      FULL_SIMP_TAC (arith_ss++holBACore_ss) [] >>
-      REPEAT STRIP_TAC >>
-      (* TODO: Use bir_exec_steps_GEN_SOME_EQ_Ended and possibly
-       * bir_exec_block_n_TO_steps_GEN *)
-      cheat,
+  Cases_on `~bir_state_is_terminated b` >- (
+    FULL_SIMP_TAC std_ss [] >>
+    Cases_on `BWS_Regular b.bst_pc.bpc_label IN ls` >| [
+      FULL_SIMP_TAC std_ss [bir_exec_to_labels_def] >>
+      IMP_RES_TAC bir_exec_to_labels_n_TO_bir_exec_block_n >>
+      IMP_RES_TAC bir_exec_to_labels_n_ended_running >>
+      EQ_TAC >| [
+        (* Case 1AI: b=ms' as assumption *)
+	DISCH_TAC >>
+	(* Rename states and clean up *)
+	rename1 `bir_exec_block_n prog st m = (l,n,c_l',b)` >>
+	rename1 `bir_exec_block_n prog st m = (l,n,c_l',st'')` >>
+	rename1 `st'' = st'` >>
+	Q.PAT_X_ASSUM `st'' = st'`
+		      (fn thm => FULL_SIMP_TAC std_ss [thm]) >>
+	(* We now have the initial state st and the final state
+         * st' *)
+	EXISTS_TAC ``m:num`` >>
+	FULL_SIMP_TAC arith_ss [] >>
+        FULL_SIMP_TAC std_ss
+          [bir_exec_block_n_to_FUNPOW_OPT_bir_trs] >>
+	REPEAT STRIP_TAC >>
+	rename1 `m' < m` >>
+	ASSUME_TAC (Q.SPECL [`prog`, `st`, `m'`]
+			    bir_exec_block_n_EXISTS) >>
+	FULL_SIMP_TAC std_ss [] >>
+	Q.EXISTS_TAC `st''` >>
+	subgoal `~bir_state_is_terminated st''` >- (
+	  IMP_RES_TAC bir_exec_block_n_block_ls_running_running
+	) >>
+	FULL_SIMP_TAC std_ss
+	  [bir_exec_block_n_to_FUNPOW_OPT_bir_trs] >>
+	(* Use bir_exec_to_labels_n_block_n_notin_ls *)
+	IMP_RES_TAC bir_exec_to_labels_n_block_n_notin_ls >>
+	REV_FULL_SIMP_TAC arith_ss [] >>
+	(* Here comes additional part for AV definitions... *)
+        FULL_SIMP_TAC std_ss [bir_ls_filter_keeps_regular],
 
-      (* Part two: Assuming bir_trs plays nice, show that b = ms' *)
-      FULL_SIMP_TAC std_ss [bir_exec_to_labels_n_def] >>
-      cheat
-    ],
-
-    (* Case 1B: Weak state counterpart of b is NOT in ls *)
-    FULL_SIMP_TAC std_ss [GSYM boolTheory.IMP_DISJ_THM] >>
-    cheat
-  ],
-
-  (* Case 2: Result of bir_exec_to_labels is Looping *)
-  (* Show that weak state of ms' cannot be in ls *)
-  FULL_SIMP_TAC std_ss [GSYM boolTheory.IMP_DISJ_THM] >>
-  cheat
-]
-);
-
-
-
-
-
-
-
-
-(*
-
-
-      Cases_on `n > 0` >| [
-        (* Number of execution steps is non-zero (regular case) *)
-        (* Also use the fact that final state is Running *)
-        subgoal
-          `FUNPOW_OPT (bir_trs prog) n ms =
-             SOME (bir_exec_infinite_steps_fun prog ms n)` >- (
-          cheat
-        ) >>
-        FULL_SIMP_TAC std_ss [bir_state_COUNT_PC_def] >>
-        Cases_on `ms'.bst_status` >> (
-          FULL_SIMP_TAC (std_ss++holBACore_ss) []
-        ) >| [
-          (* Case: Final state is Running *)
-          REPEAT STRIP_TAC >>
-          FULL_SIMP_TAC std_ss [] >>
-          QSPECL_X_ASSUM ``!n'. _`` [`n'`] >>
-          REV_FULL_SIMP_TAC std_ss [] >>
-          (* TODO: Some kind of kinduction proof on n'? *)
-          (* bir_exec_infinite_steps_fun_COUNT_PCs_EQ_0 *)
-          cheat,
-
-          (* Case: JumpOutside requires this additional
-           *       simplification *)
-          REV_FULL_SIMP_TAC (std_ss++holBACore_ss) []
-        ],
-
-	(* Number of execution steps is zero *)
-	subgoal `n = 0` >- (
+	(* Case 1AII: Assuming bir_trs plays nice, show that
+	 * b = st' (translate from bir_trs to block_n) *)
+	REPEAT STRIP_TAC >>
+	IMP_RES_TAC FUNPOW_OPT_bir_trs_to_bir_exec_block_n >>
+	rename1 `bir_exec_block_n prog st n' =
+                   (l',n'',c_l'',ms')` >>
+	rename1 `bir_exec_block_n prog st m' =
+                   (l',n'',c_l'',ms')` >>
+	rename1 `bir_exec_block_n prog st m' = (l',n',c_l'',ms')` >>
+	rename1 `bir_exec_block_n prog st m' = (l',n',c_l'',st')` >>
+	(* Here, n < n' as well as n' < n leads to contradiction, so
+	 * only remaining posssibility is n = n', which proves the
+	 * goal. *)
+	Cases_on `n' < n` >- (
+	  (* This would mean that st' does not have PC with label in
+	   * ls and pointing to instruction 0, which is a
+	   * contradiction. *)
+	  (* Step 1: Prove m' < m *)
+	  subgoal `m' < m` >- (
+	    METIS_TAC [bir_exec_block_n_step_ls]
+	  ) >>
+	  (* Step 2: Prove st'.bst_status = BST_Running *)
+	  subgoal `~bir_state_is_terminated st'` >- (
+	    IMP_RES_TAC bir_exec_block_n_step_ls_running
+	  ) >>
+	  (* Step 3: Use bir_exec_to_labels_n_block_n_notin_ls *)
+	  IMP_RES_TAC bir_exec_to_labels_n_block_n_notin_ls >>
+	  REV_FULL_SIMP_TAC arith_ss [] >>
+          FULL_SIMP_TAC std_ss [bir_ls_filter_keeps_regular]
+	) >>
+	Cases_on `n < n'` >- (
+	  (* Slightly more complex case: This would mean that
+           * state b
+	   * has crossed less than m' blocks. This would mean,
+	   * together with init assumption, that PC label of b is
+           * not in ls
+           * (with bir_exec_block_n_to_FUNPOW_OPT_bir_trs) *)
+	  subgoal `m < m'` >- (
+	    IMP_RES_TAC bir_exec_block_n_step_ls
+	  ) >>
+	  (* Use initial assumption *)
+	  QSPECL_X_ASSUM
+	    ``!n'.
+             n' < m' /\ n' > 0 ==>
+             ?ms''.
+                 (FUNPOW_OPT (bir_trs prog) n' st = SOME ms'') /\
+                 (if ~bir_state_is_terminated ms'' then
+                    BWS_Regular ms''.bst_pc.bpc_label
+                  else if ms''.bst_status = BST_AssumptionViolated then
+                    BWS_Top
+                  else BWS_Bottom) NOTIN ls`` [`m`] >>
+	  REV_FULL_SIMP_TAC arith_ss [] >>
+	  IMP_RES_TAC bir_exec_to_labels_n_ended_running >>
+	  IMP_RES_TAC bir_exec_block_n_to_FUNPOW_OPT_bir_trs >>
+	  REV_FULL_SIMP_TAC (std_ss++holBACore_ss) [] >>
+	  FULL_SIMP_TAC (std_ss++holBACore_ss) [] >>
+          REV_FULL_SIMP_TAC std_ss []
+	) >>
+	(* Since ~(n < n') and ~(n' < n), n = n' ... *)
+	subgoal `n = n'` >- (
 	  FULL_SIMP_TAC arith_ss []
 	) >>
-	FULL_SIMP_TAC (std_ss++holBACore_ss)
-		      [bir_exec_infinite_steps_fun_REWRS2,
-		       bir_state_COUNT_PC_def] >>
-	Cases_on `ms'.bst_status` >> (
-	  FULL_SIMP_TAC (std_ss++holBACore_ss) []
-	) >| [
-	  (* Case: Final state is Running *)
-	  FULL_SIMP_TAC std_ss
-	    [bir_exec_infinite_steps_fun_COUNT_PCs_def],
-
-	  (* Case: JumpOutside requires this additional
-	   *       simplification *)
-	  REV_FULL_SIMP_TAC (std_ss++holBACore_ss) []
-	]
+	subgoal `m = m'` >- (
+	  subgoal `~bir_state_is_terminated st'` >- (
+	    IMP_RES_TAC bir_exec_block_n_step_eq >>
+	    REV_FULL_SIMP_TAC arith_ss []
+	  ) >>
+	  IMP_RES_TAC bir_exec_block_n_step_eq_running
+	) >>
+	FULL_SIMP_TAC arith_ss []
       ],
 
-      REPEAT STRIP_TAC >>
-      QSPECL_X_ASSUM ``!n''. _`` [`n`] >>
-      (* TODO: What to do here??? *)
-      cheat
-    ],
+      FULL_SIMP_TAC std_ss [bir_exec_to_labels_def] >>
+      IMP_RES_TAC bir_exec_to_labels_n_ended_running >>
+      IMP_RES_TAC bir_ls_filter_keeps_regular
+    ]
+  ) >>
 
-    (* Step 1B: Weak state of b is not in ls *)
-    FULL_SIMP_TAC std_ss [GSYM boolTheory.IMP_DISJ_THM] >>
-    REPEAT STRIP_TAC >>
-    (* You can choose between two disjuncts to prove. *)
-    (* Disjunct 1: Need to prove that for all non-zero step numbers
-     * n', repeated application of bir_trs resulting in SOME state
-     * ms' (meaning, before termination) entails that ms' is not
-     * in ls'.
-     *
-     * OK, since assumptions give that Ended was reached through
-     * termination, meaning that ls' was not encountered before
-     * terminating.
-     * *)
-    (* Disjunct 2: Need to prove that there exists a non-zero step
-     * number n'' such that if repeated application of bir_trs n''
-     * times gives SOME state ms'', then ms'' is in ls'.
-     *
-     * OK, since we can give a n'' larger than the steps leading to
-     * termination, making the antecedent always false.
-     * *)
+  (* Case 1B *)
+  (* This means that Ended must have been reached by termination
+   * somewhere. *)
+  FULL_SIMP_TAC std_ss [GSYM boolTheory.IMP_DISJ_THM] >>
+  (* TODO: Previously, LHS of goal was just False here.
+   * This has to be handled differently now. *)
+  Cases_on `b.bst_status = BST_AssumptionViolated` >| [
+    cheat,
+
     cheat
   ],
 
   (* Case 2: Result of bir_exec_to_labels is Looping *)
+  FULL_SIMP_TAC std_ss [GSYM boolTheory.IMP_DISJ_THM] >>
+  REPEAT STRIP_TAC >>
+  Cases_on `~(n > 0)` >- (
+    FULL_SIMP_TAC std_ss []
+  ) >>
   FULL_SIMP_TAC std_ss [bir_exec_to_labels_def,
 			bir_exec_to_labels_n_def,
-			bir_exec_steps_GEN_EQ_Looping] >>
-  REPEAT STRIP_TAC >>
-  FULL_SIMP_TAC std_ss [GSYM boolTheory.IMP_DISJ_THM] >>
-  (* Choice of two disjuncts... *)
-(*
+			bir_exec_steps_GEN_1_EQ_Looping] >>
+  rename1 `m > 0` >>
   DISJ1_TAC >>
   REPEAT STRIP_TAC >>
-  FULL_SIMP_TAC std_ss
-    [bir_exec_infinite_steps_COUNT_STEPS_EQ_NONE] >>
-*)
-  cheat
+  IMP_RES_TAC FUNPOW_OPT_bir_trs_to_bir_exec_block_n >>
+  rename1 `bir_exec_block_n prog st m = (l',n,c_l',ms')` >>
+  rename1 `bir_exec_block_n prog st m = (l',n,c_l',st')` >>
+  QSPECL_X_ASSUM ``!(n:num). (0 < n) ==> _`` [`n`] >>
+  (* Since m is larger than zero, n has to be as well...
+   * if st is Running *)
+  subgoal `~bir_state_is_terminated st` >- (
+    QSPECL_X_ASSUM ``!(n:num). _`` [`0`] >>
+    FULL_SIMP_TAC std_ss [bir_state_is_terminated_def,
+                          bir_exec_infinite_steps_fun_REWRS]
+  ) >>
+  subgoal `0 < n` >- (
+    IMP_RES_TAC bir_exec_block_n_block_nz_init_running >>
+    FULL_SIMP_TAC arith_ss []
+  ) >>
+  FULL_SIMP_TAC arith_ss [bir_state_COUNT_PC_def] >>
+  QSPECL_X_ASSUM ``!(n:num). _`` [`n`] >>
+  subgoal `bir_exec_infinite_steps_fun prog st n = st'` >- (
+    FULL_SIMP_TAC std_ss [bir_exec_block_n_EQ_THM]
+  ) >>
+  FULL_SIMP_TAC (std_ss++holBACore_ss)
+		[bir_state_is_terminated_def] >| [
+    IMP_RES_TAC bir_exec_block_n_block_nz_final_running >>
+    REV_FULL_SIMP_TAC arith_ss [bir_state_is_terminated_def],
+
+    (* TODO: Only difference from non-AV is this case *)
+    IMP_RES_TAC bir_ls_filter_keeps_regular
+  ]
 ]
 );
-*)
-(* These could be useful: *)
-(* bir_exec_steps_GEN_SOME_EQ_Ended *)
-(* bir_exec_steps_GEN_EQ_Ended *)
-(* bir_exec_steps_GEN_change_cond_Ended_SOME *)
-(* bir_exec_steps_GEN_1_EQ_Ended *)
-(* bir_exec_to_labels_n_TO_bir_exec_block_n *)
-(* bir_exec_block_n_TO_steps_GEN *)
+
 
 val _ = export_theory();
